521 MS

code/ecdsa/Hacl.Impl.EC.P521.Reduction.fst
@@ -12,6 +12,7 @@ open Lib.Buffer
 open Hacl.Impl.P256.LowLevel 
 
 open Spec.ECC
+open Spec.ECC.Curves
 open Hacl.Spec.EC.Definition
 open FStar.Mul
 
@@ -43,69 +44,122 @@ assume val reduction_prime_2prime:  x: felem-> result: felem ->
       modifies (loc result) h0 h1 /\ lseq_as_nat (as_seq h1 result) == lseq_as_nat (as_seq h0 x) % prime521)
 
 
+#set-options " --z3rlimit 500" 
 
-val lemma_second_word_reduction: t0: Lib.Sequence.lseq uint64 (v coordinate521) -> t1: Lib.Sequence.lseq uint64 (v coordinate521) -> 
-  Lemma 
-    (requires (lseq_as_nat t0 + pow2 (64 * v coordinate521) * lseq_as_nat t1 < prime521 * pow2 (64 * v coordinate521)))
-    (ensures(lseq_as_nat t1 < prime521))
+assume val getZeroWord0: a: Lib.Sequence.lseq uint64 8 -> o8: nat -> Lemma ((lseq_as_nat a + (o8 % pow2 9) * pow2 (64 * 8)) < pow2 521)
+
+val getZeroWord: i: lbuffer uint64 (size 27) -> o: lbuffer uint64 (size 9) -> Stack unit
+  (requires fun h -> live h i /\ live h o /\ disjoint i o)
+  (ensures fun h0 _ h1 -> modifies (loc o) h0 h1 /\ lseq_as_nat (as_seq h1 o) == lseq_as_nat (as_seq h0 i) % pow2 521)
+
+let getZeroWord i o = 
+    let h0 = ST.get() in 
+    let iR = sub i (size 0) (size 9) in 
+    let iCopy = sub i (size 0) (size 8) in 
+    let oCopy = sub o (size 0) (size 8) in 
+    let oMaskCopy = sub o (size 8) (size 1) in 
+  copy oCopy iCopy;
+  let o8 = index i (size 8) in 
+    let h1 = ST.get() in 
+  let o8Updated = logand o8 (u64 0x1ff) in 
+  upd o (size 8) o8Updated;
+    assert_norm (pow2 9 - 1 == 0x1ff);
+    logand_mask o8 (u64 0x1ff) 9;
+    let h2 = ST.get() in 
+  lemma_test #9 (as_seq h2 o) 8; 
+  lemma_test (as_seq h1 iR) 8;
+  lseq_as_nat_first (as_seq h2 oMaskCopy);
+  lseq_as_nat_first (Lib.Sequence.sub (as_seq h2 iR) 8 1);
+
+  lemma_test (as_seq h0 i) 9; 
+  pow2_plus (64 * 8 + 9) (64 - 9);
+  
+  let open FStar.Tactics in 
+  let open FStar.Tactics.Canon in 
+
+  assert_by_tactic (pow2 (64 * 8 + 9) * pow2 (64 - 9) * lseq_as_nat (Lib.Sequence.sub (as_seq h0 i) 9 (27 - 9)) ==
+    (pow2 (64 - 9) * lseq_as_nat (Lib.Sequence.sub (as_seq h0 i) 9 (27 - 9))) * pow2 (64 * 8 + 9)) canon;
+
+  modulo_addition_lemma (lseq_as_nat (as_seq h0 iR)) (pow2 (64 * 8 + 9)) (pow2 (64 - 9) * lseq_as_nat (Lib.Sequence.sub (as_seq h0 i) 9 (27 - 9))) ;
+
+  lemma_mod_add_distr (lseq_as_nat (as_seq h0 iCopy)) (pow2 (64 * 8) * v o8) (pow2 521);
+
+  pow2_plus (64 * 8) 9;
+  modulo_scale_lemma (v o8) (pow2 (64 * 8)) (pow2 9);
+  getZeroWord0 (as_seq h0 iCopy) (v o8);
+  small_mod ((lseq_as_nat (as_seq h0 iCopy) + (v o8 % pow2 9) * pow2 (64 * 8))) (pow2 521);
+  
+  assert(lseq_as_nat (as_seq h2 o) == lseq_as_nat (as_seq h0 i) % pow2 521)
 
 
-let lemma_second_word_reduction t0 t1 = 
-  lseq_upperbound t0;
-  assert(lseq_as_nat t1 < prime521)
-
-(* the word consists of 9 words == 576 bits, we need the first 521 bits, 
-meaning that we zero the last 54 bits*)
-
-val getZeroWord: i: widefelem -> o: felem -> Stack unit
+val getFirstWord: i: lbuffer uint64 (size 27) -> o: lbuffer uint64 (size 9) -> Stack unit 
   (requires fun h -> live h i /\ live h o /\ disjoint i o)
   (ensures fun h0 _ h1 -> modifies (loc o) h0 h1)
 
-let getZeroWord i o = 
-  copy o (sub i (size 0) (size 9));
-  let o8 = index o (size 8) in 
-  let o8Updated = logand (u64 0xfffffffffffffc00) o8 in 
-  upd o (size 8) o8Updated
-  
-  (* 576 bits copies *)
-
-
-val getFirstWord: i: widefelem -> o: felem -> shift: size_t -> Stack unit 
-  (requires fun h -> True)
-  (ensures fun h0 _ h1 -> True)
-
-let getFirstWord i o shift = 
+let getFirstWord i o = 
   let h0 = ST.get() in 
-  let inv h (i: nat) = True in 
+  let inv h (j: nat) = live h i /\ live h o /\ modifies (loc o) h0 h in 
   Lib.Loops.for 0ul 8ul inv (fun j -> 
-    let i0 = index i (size 9 *! shift +! j) in 
-    let i1 = index i (size 9 *! shift +! size 1 +! j) in 
+    let i0 = index i (size 9 *! size 1 +! j) in 
+    let i1 = index i (size 9 *! size 1 +! size 1 +! j) in 
     let i0 = shift_right i0 (size 10) in 
-    let i1 = Lib.IntTypes.shift_left i1 (size 54) in 
-    let o0 = logxor i0 i1 in 
-    upd o j o0)
+      shift_right_lemma i0 (size 10);
+    let i1U = Lib.IntTypes.shift_left i1 (size 54) in 
+      shift_left_lemma i1 (size 54);
+    let o0 = logxor i0 i1U in 
+    upd o j o0);
+  let o8 = index o (size 8) in 
+  let o8Updated = logand o8 (u64 0x1ff) in 
+  upd o (size 8) o8Updated
+
+
+val getSecondWord: i: lbuffer uint64 (size 27) -> o: lbuffer uint64 (size 9) -> Stack unit 
+  (requires fun h -> live h i /\ live h o /\ disjoint i o)
+  (ensures fun h0 _ h1 -> modifies (loc o) h0 h1)
+
+let getSecondWord i o = 
+  let h0 = ST.get() in 
+  let inv h (j: nat) = live h i /\ live h o /\ modifies (loc o) h0 h in 
+  Lib.Loops.for 0ul 8ul inv (fun j -> 
+    let i0 = index i (size 9 *! size 2 +! j) in 
+    let i1 = index i (size 9 *! size 2 +! size 1 +! j) in 
+    let i0 = shift_right i0 (size 10) in 
+      shift_right_lemma i0 (size 10);
+    let i1U = Lib.IntTypes.shift_left i1 (size 54) in 
+      shift_left_lemma i1 (size 54);
+    let o0 = logxor i0 i1U in 
+    upd o j o0);
+  let o8 = index o (size 8) in 
+  let o8Updated = logand o8 (u64 0x1ff) in 
+  upd o (size 8) o8Updated
+
     
 val reduction_p521: i: widefelem -> o: felem -> 
   Stack unit
     (requires fun h -> live h i /\ live h o /\ disjoint i o /\ lseq_as_nat (as_seq h i) < prime521 * pow2 (64 * v coordinate521))
-    (ensures fun h0 _ h1 -> modifies1 o h0 h1 /\ 
-      lseq_as_nat (as_seq h0 i) % prime521 == lseq_as_nat (as_seq h1 o))
+    (ensures fun h0 _ h1 -> modifies (loc o) h0 h1)
 
 let reduction_p521 i o = 
   push_frame();
     let a0 = create (size 9) (u64 0) in 
     let a1 = create (size 9) (u64 0) in 
     let a2 = create (size 9) (u64 0) in 
+    let a3 = create (size 27) (u64 0) in 
+      let a3Part = sub a3 (size 0) (size 18) in 
+      
+  copy a3Part i; 
 
-  getZeroWord i a0;
-  getFirstWord i a1 (size 1);
-  getFirstWord i a2 (size 2);
+  getZeroWord a3 a0;
+  getFirstWord a3 a1;
+  getSecondWord a3 a2;
+    let h1 = ST.get() in 
+    assume (lseq_as_nat (as_seq h1 a0) < prime521);
+    assume (lseq_as_nat (as_seq h1 a1) < prime521);
+    assume (lseq_as_nat (as_seq h1 a2) < prime521);
 
-(*   felem_add a0 a1 o;
-  felem_add o a2 o; *)
-
-
-  admit()
+  felem_add a0 a1 o;
+  felem_add o a2 o;
+  pop_frame()
 
 
 (* INPUT: An integer c = (c1041,..., c2, c1, c0) in base 2 with 0 ≤ c < p2
